style: refine custom syntax for de Bruijn indices

Plfl/DeBruijn.lean
@@ -39,18 +39,18 @@ end Context
 inductive Lookup : Context → Ty → Type where
 | z : Lookup (Γ :< t) t
 | s : Lookup Γ t → Lookup (Γ :< t') t
-deriving DecidableEq
+deriving DecidableEq, Repr
 
 namespace Lookup
   infix:40 " ∋ " => Lookup
 
-  def getElem {Γ : Context} (n : Fin (Γ.length)) : Γ ∋ Γ[n] :=
-    match Γ, n with
-    | _ :: _, ⟨0, _⟩ => .z
-    | _ :: _, ⟨n + 1, h⟩ => .s (getElem ⟨n, Nat.le_of_succ_le_succ h⟩)
-
   -- https://github.com/arthurpaulino/lean4-metaprogramming-book/blob/d6a227a63c55bf13d49d443f47c54c7a500ea27b/md/main/macros.md#simplifying-macro-declaration
-  macro " ♯ " n:term:90 : term => `(getElem ⟨$n, by trivial⟩)
+  syntax "get_elem" (ppSpace term) : tactic
+  macro_rules | `(tactic| get_elem $n) => match n.1.toNat with
+  | 0 => `(tactic | exact Lookup.z)
+  | n+1 => `(tactic| apply Lookup.s; get_elem $(Lean.quote n))
+
+  macro " ♯ " n:term:90 : term => `(by get_elem $n)
 
   example : ∅ :< ℕt =⇒ ℕt :< ℕt ∋ ℕt := .z
   example : ∅ :< ℕt =⇒ ℕt :< ℕt ∋ ℕt := ♯0
@@ -70,21 +70,58 @@ inductive Term : Context → Ty → Type where
 | succ : Term Γ ℕt → Term Γ ℕt
 | case : Term Γ ℕt → Term Γ a → Term (Γ :< ℕt) a → Term Γ a
 | mu : Term (Γ :< a) a → Term Γ a
-deriving DecidableEq
+deriving DecidableEq, Repr
 
 namespace Term
   infix:40 " ⊢ " => Term
 
   prefix:50 " ƛ " => lam
   prefix:50 " μ " => mu
-  notation:max " 𝟘? " e " [zero: " o " |succ " n " : " i " ] " => case e o n i
+  notation " 𝟘? " => case
   infixr:min " $ " => ap
   infixl:70 " □ " => ap
   prefix:80 " ι " => succ
   prefix:90 " ` " => var
   notation " 𝟘 " => zero
 
-  example : ∅ :< ℕt =⇒ ℕt :< ℕt ⊢ ℕt := `♯0
-  example : ∅ :< ℕt =⇒ ℕt :< ℕt ⊢ ℕt =⇒ ℕt := `♯1
-  example : ∅ :< ℕt =⇒ ℕt :< ℕt ⊢ ℕt := `♯1 □ `♯0
+  -- https://plfa.github.io/DeBruijn/#abbreviating-de-bruijn-indices
+  macro " # " n:term:90 : term => `(`♯$n)
+
+  example : ∅ :< ℕt =⇒ ℕt :< ℕt ⊢ ℕt := #0
+  example : ∅ :< ℕt =⇒ ℕt :< ℕt ⊢ ℕt =⇒ ℕt := #1
+  example : ∅ :< ℕt =⇒ ℕt :< ℕt ⊢ ℕt := #1 $ #0
+  example : ∅ :< ℕt =⇒ ℕt :< ℕt ⊢ ℕt := #1 $ #1 $ #0
+  example : ∅ :< ℕt =⇒ ℕt ⊢ ℕt =⇒ ℕt := ƛ (#1 $ #1 $ #0)
+  example : ∅ ⊢ (ℕt =⇒ ℕt) =⇒ ℕt =⇒ ℕt := ƛ ƛ (#1 $ #1 $ #0)
+
+  @[simp]
+  def ofNat : ℕ → Term Γ ℕt
+  | 0 => zero
+  | n + 1 => succ <| ofNat n
+
+  instance : Coe ℕ (Term Γ ℕt) where coe := ofNat
+  instance : OfNat (Term Γ ℕt) n where ofNat := ofNat n
+
+  -- https://plfa.github.io/DeBruijn/#test-examples
+  example : Γ ⊢ ℕt := ι ι 𝟘
+  example : Γ ⊢ ℕt := 2
+
+  abbrev add : Γ ⊢ ℕt =⇒ ℕt =⇒ ℕt := μ ƛ ƛ (𝟘? (#1) (#0) (ι (#3 □ #0 □ #1)))
+
+  example : Γ ⊢ ℕt := add □ 2 □ 2
+
+  /--
+  The Church numeral Ty.
+  -/
+  abbrev Ch (t : Ty) : Ty := (t =⇒ t) =⇒ t =⇒ t
+
+  abbrev succC : Γ ⊢ ℕt =⇒ ℕt := ƛ #0
+  abbrev twoC : Γ ⊢ Ch a := ƛ ƛ (#1 $ #1 $ #0)
+  abbrev addC : Γ ⊢ Ch a =⇒ Ch a =⇒ Ch a := ƛ ƛ ƛ ƛ (#3 □ #1 $ #2 □ #1 □ #0)
+  example : Γ ⊢ ℕt := addC □ twoC □ twoC □ succC □ 𝟘
+
+  -- https://plfa.github.io/DeBruijn/#exercise-mul-recommended
+  abbrev mulC : Γ ⊢ Ch a =⇒ Ch a =⇒ Ch a := ƛ ƛ ƛ ƛ (#3 □ (#2 □ #1) □ #0)
 end Term
+
+-- https://plfa.github.io/DeBruijn/#renaming
